Prove pointer rules for unary heap version

src/UnaryHeap.v
@@ -3,6 +3,7 @@ From Coq Require Import
   Arith.PeanoNat
   Logic.FunctionalExtensionality
   Lists.List
+  Classes.Morphisms
   Lia.
 
 From Heapster Require Import
@@ -294,7 +295,7 @@ Section HeapPerms.
       apply Hlte in H'. destruct H' as (Hprep & Hpreno_err & Hsep).
       destruct (typing_multistep _ _ _ Htyping _ _ Hp Hprep _ _ Hmultistep) as (P' & Htyping' & p' & Hp' & Hsep_step & Hprep').
       eapply (typing_soundness_step _ _ _ Htyping').
-      3: apply Hstep. (* apply H10 in H7. simpl. *)
+      3: apply Hstep.
       exists p', no_error_perm. split; [| split; [| split]]; cbn; auto; try reflexivity.
       apply Hsep_step in Hsep. eapply separate_upwards_closed; eauto.
       split; [| split]; auto.
@@ -302,178 +303,196 @@ Section HeapPerms.
       apply IHHmultistep; eauto.
   Qed.
 
-
-  (*** TODO *)
-  Program Definition read_perm (ptr : addr) (v : Value) : perm :=
+  Program Definition read_perm (ptr : addr) (v : Value) : @perm config :=
     {|
-      (* ptr points to valid memory *)
-      pre x := read x ptr = Some v;
-      (* only checks if the memory ptr points to in the 2 configs are equal *)
-      rely x y := read x ptr = read y ptr;
-      (* no updates allowed *)
+      (** [ptr] points to [v] *)
+      pre x := read (m x) ptr = Some v;
+      (** only checks if the memory [ptr] points to in the 2 memories are equal *)
+      rely x y := read (m x) ptr = read (m y) ptr;
+      (** no updates allowed *)
       guar x y := x = y;
     |}.
   Next Obligation.
-    constructor; repeat intro; auto. etransitivity; eauto.
+    constructor; [intros [] | intros [] [] []]; auto; etransitivity; eauto.
   Qed.
 
-  Program Definition write_perm (ptr : addr) (v : SByte) : perm :=
+  Program Definition write_perm (ptr : addr) (v : Value) : @perm config :=
     {|
-      (* ptr points to valid memory *)
-      pre x := read x ptr = Some v;
-      (* only checks if the memory ptr points to in the 2 configs are equal *)
-      rely x y := read x ptr = read y ptr;
+      (* [ptr] points to [v] *)
+      pre x := Some v = read (m x) ptr;
+      (* only checks if the memory [ptr] points to in the 2 configs are equal *)
+      rely x y := read (m x) ptr = read (m y) ptr;
       (* only the pointer we have write permission to may change *)
-      guar x y := (forall ptr', ptr <> ptr' -> read x ptr' = read y ptr') /\
-                    alloc_invariant x y ptr /\
-                    e x = e y;
+      guar x y :=
+        (e x = e y) /\
+          (forall ptr', ptr <> ptr' -> read (m x) ptr' = read (m y) ptr') /\
+          (forall ptr', sizeof (m x) ptr' = sizeof (m y) ptr') /\
+          length (m x) = length (m y);
     |}.
   Next Obligation.
-    constructor; repeat intro; auto. etransitivity; eauto.
+    constructor; [intros [] | intros [] [] []]; auto; etransitivity; eauto.
   Qed.
   Next Obligation.
-    constructor; split; repeat intro; try solve [intuition].
-    - split; [| split]; reflexivity.
-    - destruct H, H0. etransitivity. apply H; auto. auto.
-    - destruct H as (? & ? & ? & ?), H0 as (? & ? & ? & ?).
-      split; [| split]; etransitivity; eauto.
+    constructor; [intros [] |]; auto.
+    - intros [] [] [] [] []. split.
+      + destruct H, H1. subst. eexists.
+      + split; [| split]; (etransitivity; [apply H0; auto |]); apply H2; auto.
   Qed.
 
-  Definition read_Perms (ptr : addr) (P : SByte -> Perms) : Perms :=
-    meet_Perms (fun Q => exists y : SByte, Q = singleton_Perms (read_perm ptr y) ** P y).
-
-  Definition write_Perms (ptr : addr) (P : SByte -> Perms) : Perms :=
-    meet_Perms (fun Q => exists y : SByte, Q = singleton_Perms (write_perm ptr y) ** P y).
-
-
-  Variant typing_gen {R} typing (P : Perms) (Q : R -> Perms) : itree E R -> Prop :=
-  | cond : forall t, (exists c t' c', step t c t' c') /\ (* we can step *)
-                (forall p c, p ∈ P ->
-                        pre p c ->
-                        forall t' c',
-                          step t c t' c' -> (* and everything we can step to... *)
-                          (
-                            (* we step to configs that satisfy the perm *)
-                            guar p c c' /\
-                            (* we step to machines that are well-typed by some other perm that maintains separation *)
-                            exists P', typing P' Q t' /\ exists p', p' ∈ P' /\ sep_step p p' /\ pre p' c')) ->
-                typing_gen typing P Q t
-    | ret : forall r, P ⊑ Q r -> typing_gen typing P Q (Ret r).
-
-  Lemma typing_gen_mon {R} : monotone3 (@typing_gen R).
+  Lemma sep_step_read_perm l v v' :
+    sep_step (read_perm l v) (read_perm l v').
   Proof.
-    repeat intro.
-    inversion IN; subst.
-    - econstructor. destruct H. split; auto.
-      intros. edestruct H0; eauto. split; eauto.
-      destruct H5 as (? & ? & (? & ? & ? & ?)). eexists. split; eauto.
-    - constructor 2; auto.
+    repeat intro. split; apply H; auto.
   Qed.
-  Hint Resolve typing_gen_mon : paco.
 
-  Definition typing {R} := paco3 (@typing_gen R) bot3.
+  Lemma sep_step_write_perm l v v' :
+    sep_step (write_perm l v) (write_perm l v').
+  Proof.
+    repeat intro. split; apply H; auto.
+  Qed.
 
-  Example typing_ex_updown :
-    typing ex_updown_Perms (fun _ => ex_updown_Perms_b (Z.of_nat 1)) (trigger (Store (Z.of_nat 1))).
+  Lemma read_separate ptr ptr' v v' :
+    read_perm ptr v ⊥ read_perm ptr' v'.
+  Proof.
+    split; intros; auto; destruct x, y; cbn in *; inversion H; auto.
+  Qed.
+
+  Lemma read_lte_write : forall ptr v, write_perm ptr v <= read_perm ptr v.
+  Proof.
+    constructor; cbn; intros [] []; subst; auto.
+    intros []; subst.
+    split; [| split; [| split]]; try reflexivity.
+  Qed.
+
+  Lemma write_write_sep ptr ptr' v v' :
+      ptr <> ptr' ->
+      write_perm ptr v ⊥ write_perm ptr' v'.
+  Proof.
+    intros Hdiff. constructor; intros; destruct x, y; cbn; apply H; auto.
+  Qed.
+
+  Definition read_Perms (ptr : addr) (P : Value -> Perms) : Perms :=
+    join_Perms (fun Q => exists y : Value, Q = singleton_Perms (read_perm ptr y) * P y).
+
+  Definition write_Perms (ptr : addr) (P : Value -> Perms) : Perms :=
+    join_Perms (fun Q => exists y : Value, Q = singleton_Perms (write_perm ptr y) * P y).
+
+  Program Definition eqp {A} (a a' : A) : @Perms config :=
+    {|
+      in_Perms _ := a = a'
+    |}.
+
+  (*** TODO EQP RULES *)
+
+  Lemma typing_load ptr (Q : Value -> Perms) :
+    typing
+      (read_Perms ptr Q)
+      (fun x => (read_Perms ptr (eqp x)) * Q x)
+      (trigger (Load (VPtr ptr))).
   Proof.
     pstep. constructor 1. split.
-    { exists (Z.of_nat 0), (Ret tt), (Z.of_nat 1). constructor. }
-    intros p c (? & (b & ?) & Hp) Hpre t' c' Hstep.
-    inversion Hstep; subst. apply Eqdep.EqdepTheory.inj_pair2 in H2. subst. split.
-    - apply Hp. cbn. auto.
-    - exists (ex_updown_Perms_b (Z.of_nat 1)). split.
-      + left. pstep. constructor 2. reflexivity.
-      + exists (ex_updown_perm (Z.of_nat 1)). split; [| split]; cbn; auto. reflexivity.
-        eapply sep_step_lte. apply Hp.
-        apply sep_step_rg; intros; auto.
+    - eexists {| m := _; e := false |}. do 2 eexists.
+      constructor. unfold read'. cbn. eapply read_mem_at.
+      Unshelve. apply (VNum 0).
+    - intros p' c (P & (v & ?) & Hp) Hpre t' c' Hstep. subst.
+      destruct Hp as (p & q & Hp & Hq & Hsep & Hlte). cbn in Hp.
+      inversion Hstep; subst; apply Eqdep.EqdepTheory.inj_pair2 in H1; subst.
+      + split; intuition. assert (v = v0). {
+          apply Hlte in Hpre. destruct Hpre as (Hpre & _). apply Hp in Hpre.
+          rewrite Hpre in H4. inversion H4. auto.
+        } subst. eexists. split.
+        * left. pstep. constructor 2. reflexivity.
+        * exists (p ** q). split; [| split]; eauto.
+          2: { eapply sep_step_lte. 2: reflexivity. auto. }
+          exists p, q. split; [| split]; intuition.
+          eexists. split. eexists. reflexivity. cbn. eexists. exists top_perm.
+          split; [| split; [| split]]; eauto. apply separate_top. apply sep_conj_perm_top.
+      + apply Hlte in Hpre. destruct Hpre as (Hpre & _). apply Hp in Hpre.
+        rewrite Hpre in H4. inversion H4.
   Qed.
 
-  Lemma rewrite_spin {R} : (ITree.spin : itree E R) = Tau (ITree.spin).
+  Lemma typing_store_alt {R} ptr val (P Q : Value -> Perms) (r : R) :
+    typing
+      (write_Perms ptr P * Q val)
+      (fun _ => write_Perms ptr Q)
+      (vis (Store (VPtr ptr) val) (fun _ => Ret tt)).
   Proof.
-    intros. apply bisimulation_is_eq.
-    ginit. gcofix CIH. gstep. unfold ITree.spin. constructor.
-    apply Reflexive_eqit_gen_eq.
-  Qed.
-  Example typing_spin {R} : forall P Q, typing P Q (ITree.spin : itree E R).
-  Proof.
-    pcofix CIH. intros. pstep. constructor 1. split.
-    - exists (Z.of_nat 0). eexists. exists (Z.of_nat 0). rewrite rewrite_spin. constructor.
-    - intros. rewrite rewrite_spin in H1. inversion H1; subst; split; intuition.
-      exists P. split.
-      + right. auto.
-      + exists p; split; [| split]; intuition.
-  Qed.
-
-  Lemma typing_lte {R} : forall P P' Q Q' (t : itree E R),
-      typing P Q t ->
-      P' ⊑ P ->
-      (forall r, Q r ⊑ Q' r) ->
-      typing P' Q' t.
-  Proof.
-    pcofix CIH. intros. pstep. pinversion H0; subst.
-    - constructor 1. destruct H. split; auto. intros.
-      edestruct H3; eauto. split; auto.
-      destruct H8 as (? & ? & (? & ? & ? & ?)). pclearbot.
-      eexists; split.
-      + right. eapply CIH; eauto. reflexivity.
-      + eexists. split; [| split]; eauto.
-    - constructor 2. etransitivity; eauto. etransitivity; eauto.
-  Qed.
-
-  Lemma typing_bind {R1 R2} : forall P Q R (t : itree E R1) (k : R1 -> itree E R2),
-      typing P Q t ->
-      (forall r1, typing (Q r1) R (k r1)) ->
-      typing P R (x <- t;; k x).
-  Proof.
-    pcofix CIH. intros. pinversion H0; subst.
-    - destruct H as ((c & t' & c' & Hstep) & ?). pstep. constructor. split; auto.
-      { do 3 eexists. apply step_bind; eauto. }
-      intros. inversion H4; subst.
-      + pose proof @eqitree_inv_bind_tau.
-        edestruct H5 as [(? & ? & ?) | (? & ? & ?)]; [rewrite H6; reflexivity | |];
-          apply bisimulation_is_eq in H7; apply bisimulation_is_eq in H8; subst;
-          [| inversion Hstep].
-        destruct (H _ _ H2 H3 _ _ (step_tau _ _)) as (? & P' & ? & (p' & ? & ? & ?)).
-        pclearbot. split; auto. exists P'. split; eauto.
-      + pose proof @eqitree_inv_bind_vis.
-        edestruct H5 as [(? & ? & ?) | (? & ? & ?)]; [rewrite H6; reflexivity | |];
-          apply bisimulation_is_eq in H7; subst; [| inversion Hstep].
-        rewritebisim_in @bind_vis H6. inversion H6. apply Eqdep.EqdepTheory.inj_pair2 in H9; subst.
-        destruct (H _ _ H2 H3 _ _ (step_load _ _)) as (? & P' & ? & (p' & ? & ? & ?)).
-        pclearbot. split; auto. exists P'. split; eauto.
-      + pose proof @eqitree_inv_bind_vis.
-        edestruct H5 as [(? & ? & ?) | (? & ? & ?)]; [rewrite H6; reflexivity | |];
-          apply bisimulation_is_eq in H7; subst; [| inversion Hstep].
-        rewritebisim_in @bind_vis H6. inversion H6. apply Eqdep.EqdepTheory.inj_pair2 in H9; subst.
-        destruct (H _ _ H2 H3 _ _ (step_store _ _ _)) as (? & P' & ? & (p' & ? & ? & ?)).
-        pclearbot. split; auto. exists P'. split; eauto.
-    - rewritebisim @bind_ret_l. eapply paco3_mon_bot; eauto. eapply typing_lte; eauto.
-      reflexivity.
-  Qed.
-
-  Lemma typing_perm_frame {R : Type} : forall P Q P' (t : itree E R),
-      typing P Q t ->
-      typing (P * P') (fun r => Q r * P') t.
-  Proof.
-    pcofix CIH. intros. pinversion H0; subst.
-    - pstep. constructor 1. split.
-      { destruct H as ((c & t' & c' & Hstep) & ?).
-        do 3 eexists; eauto. }
-      destruct H as (_ & H).
-      intros pp c (p & p' & Hp & Hp' & Hsep & Hpp) Hpre t' c' Hstep.
-      edestruct H; eauto.
-      { apply Hpp. apply Hpre. }
+  pstep. constructor 1. split.
+  - eexists {| m := _; e := false |}. do 2 eexists.
+    constructor. unfold write'. cbn.
+    rewrite write_mem_at. reflexivity. Unshelve. apply (VNum 0).
+  - intros p'' c (p' & q & (? & (val' & ?) & Hp') & Hq & Hsep'' & Hlte'') Hpre t' c' Hstep. subst.
+    destruct Hp' as (pw & p & Hwrite & Hp & Hsep' & Hlte'). cbn in Hwrite.
+    inversion Hstep; subst; apply Eqdep.EqdepTheory.inj_pair2 in H2; subst.
+    {
+      assert (guar p' c c').
+      {
+        unfold write' in H5. destruct (write (m c) ptr val) eqn:Hwrite'; inversion H5.
+        apply Hlte'. constructor 1. left. apply Hwrite.
+        split; [| split; [| split]]; auto.
+        - eapply write_success_read_neq; eauto.
+        - eapply write_success_sizeof; eauto.
+        - eapply write_success_length; eauto.
+      }
       split.
-      { apply Hpp. constructor. left. assumption. }
-      destruct H2 as (P'' & Ht' & p'' & Hpp' & Hsep_step & Hpre').
-      exists (P'' * P'). pclearbot. split; auto.
-      exists (p'' ** p'). split; [| split].
-      + apply sep_conj_Perms_perm; auto.
-      + eapply sep_step_lte; eauto. eapply sep_step_sep_conj_l; auto.
-      + split; [| split]; auto.
-        apply Hpp in Hpre. destruct Hpre as (? & ? & ?). respects.
-        apply H4; auto.
-    - pstep. constructor 2. apply sep_conj_Perms_monotone; intuition.
+      { apply Hlte''. constructor 1. left. auto. }
+      eexists. split.
+      { left. pstep. constructor 2. reflexivity. }
+      exists (write_perm ptr val ** q). split; [| split].
+      - eexists. split; eauto.
+        do 2 eexists. split; [| split; [apply Hq | split]]; cbn; try reflexivity.
+        symmetry in Hsep''. eapply separate_upwards_closed in Hsep''; eauto.
+        apply separate_sep_conj_perm_l in Hsep''.
+        eapply separate_upwards_closed in Hsep''; eauto.
+        symmetry. split; apply Hsep''.
+      - eapply sep_step_lte; eauto. apply sep_step_sep_conj_l.
+        { apply Hlte'' in Hpre. apply Hpre. }
+        eapply sep_step_lte; eauto. eapply sep_step_lte. apply lte_l_sep_conj_perm.
+        eapply sep_step_lte; eauto.
+        apply sep_step_write_perm.
+      - cbn. split; [| split]; auto.
+        + unfold write' in H5. destruct (write (m c) ptr val) eqn:Hwrite'; inversion H5.
+          destruct c'. inversion H1. subst. cbn.
+          apply write_success_read_eq in Hwrite'.
+          symmetry. assumption.
+        + respects. 2: { apply Hlte'' in Hpre. apply Hpre. }
+                  apply Hlte'' in Hpre. apply Hpre. auto.
+        + apply Hlte'' in Hpre. destruct Hpre as (_ & _ & Hsep). symmetry in Hsep.
+          eapply separate_upwards_closed in Hsep; eauto.
+          apply separate_sep_conj_perm_l in Hsep.
+          eapply separate_upwards_closed in Hsep; eauto. destruct Hsep. constructor; auto.
+    }
+    {
+      apply Hlte'' in Hpre. destruct Hpre as (? & _).
+      apply Hlte' in H. destruct H as (? & _).
+      apply Hwrite in H. cbn in H.
+      unfold write' in H5.
+      symmetry in H. apply read_success_write with (v' := val) in H. destruct H.
+      rewrite H in H5. inversion H5.
+    }
   Qed.
 
-End IntPerms.
+  Instance Proper_eq_Perms_typing {R} : Proper (eq_Perms ==> (pointwise_relation _ eq_Perms) ==> eq ==> flip impl) (@typing R).
+  Proof.
+    pcofix CIH. repeat intro. subst. pstep. pinversion H3; subst.
+    - constructor 1. destruct H. split; auto. intros.
+      edestruct H2; eauto. rewrite <- H0; auto. split; auto.
+      destruct H8 as (? & ? & ? & ? & ? & ?). eexists. split.
+      right. pclearbot. eapply CIH. 3: reflexivity. 3: apply H8.
+      reflexivity. auto. eauto.
+    - constructor 2; eauto. rewrite H0. rewrite H1. auto.
+  Qed.
+
+  Lemma typing_store {R} ptr val (P Q : Value -> @Perms config) (r : R) :
+    typing
+      (write_Perms ptr P)
+      (fun _ => write_Perms ptr (eqp val))
+      (vis (Store (VPtr ptr) val) (fun _ => Ret tt)).
+  Proof.
+    assert (top_Perms ≡ eqp val val).
+    { split; repeat intro; cbn; auto. }
+    rewrite <- sep_conj_Perms_top_identity. rewrite sep_conj_Perms_commut.
+    rewrite H. eapply typing_store_alt; eauto.
+  Qed.
+
+End HeapPerms.
